Porting the tests + improvements
- perm_left and perm_right don't drop emp anymore

tests/demo/A_hpp_spec.v
@@ -10,31 +10,29 @@ Require Import Coq.Strings.String.
 Local Open Scope Z_scope.
 Local Open Scope string_scope.
 
+Require Import Cpp.Auto.
 Require Demo.A_hpp.
 
 Section with_Σ.
 Context {Σ:gFunctors}.
 
-Local Notation function_spec := (function_spec Σ) (only parsing).
+Local Notation mpred := (mpred Σ) (only parsing).
 
-Definition A__foo := "_ZN1A3fooEi".
-Definition A__foo_spec : function_spec :=
-  SFunction (Qmut T_int) (Qmut T_int :: nil)
-      (fun x =>
+Definition A__foo_spec : mpred := ltac:(
+  specify (name "::A::foo") A_hpp.module
+      uconstr:(fun x =>
          \with (y : Z)
          \pre [| x = Vint y |] ** [| has_type (y + 6) T_int |]
-         \post [r] [| r = Vint (y + 6)%Z |]).
+         \post [r] [| r = Vint (y + 6)%Z |])).
 
-Definition A__bar := "_ZN1A3barEi".
-Definition A__bar_spec : function_spec :=
-  SFunction (Qmut T_int) (Qmut T_int :: nil)
-      (fun x =>
+Definition A__bar_spec : mpred := ltac:(
+  specify (name "::A::bar") A_hpp.module
+      uconstr:(fun x =>
          \with (y : Z)
          \pre [| x = Vint y |] ** [| has_type (y + 7) T_int |]
-         \post [r] [| r = Vint (y + 7)%Z |]).
+         \post [r] [| r = Vint (y + 7)%Z |])).
 
-Definition A_hpp_spec (resolve : _) :=
-  module (ti_cglob (resolve:=resolve) A__foo A__foo_spec)
-         (ti_cglob (resolve:=resolve) A__bar A__bar_spec).
+Definition A_hpp_spec :=
+  module A__foo_spec A__bar_spec.
 
 End with_Σ.
